beta/imports.v
@@ -3,7 +3,7 @@ From Coq Require Export Logic.PropExtensionality
   (propositional_extensionality) Program.Basics (const) FunInd.
 From Equations Require Export Equations.
 From Hammer Require Export Tactics.
-From stdpp Require Export relations (rtc, rtc_transitive, rtc_once, rtc_inv, rtc(..), diamond, confluent, diamond_confluent).
+From stdpp Require Export relations (rtc, rtc_transitive, rtc_once, rtc_inv, rtc(..), diamond, confluent, diamond_confluent) base(sum_relation(..)).
 Require Export Psatz.
 
 Global Set Warnings "-notation-overridden".
